make src2imp hold "option impvar" so that deltas and mappings use the same type, but it seems deltas would need a "remove by value" function too?

compiler/src/RegAlloc_delta_checker.v
@@ -13,7 +13,7 @@ Require Import bedrock2.Syntax.
 Require Import compiler.util.ListLib.
 Require Import compiler.Simp.
 Require Import compiler.Simulation.
-
+Require Import bedrock2.MetricLogging.
 
 Local Notation "'bind_opt' x <- a ; f" :=
   (match a with
@@ -23,6 +23,29 @@ Local Notation "'bind_opt' x <- a ; f" :=
   (right associativity, at level 70, x pattern).
 
 Axiom TODO_sam: False.
+
+Section TooVerbose.
+  Context {p1 p2: Semantics.parameters}.
+  Variable exec1:
+     @Semantics.trace p1 -> @Semantics.mem p1 -> @Semantics.locals p1 -> MetricLog ->
+    (@Semantics.trace p1 -> @Semantics.mem p1 -> @Semantics.locals p1 -> MetricLog -> Prop) ->
+    Prop.
+  Variable exec2:
+     @Semantics.trace p2 -> @Semantics.mem p2 -> @Semantics.locals p2 -> MetricLog ->
+    (@Semantics.trace p2 -> @Semantics.mem p2 -> @Semantics.locals p2 -> MetricLog -> Prop) ->
+    Prop.
+  Variable related:
+             @Semantics.trace p1 -> @Semantics.mem p1 -> @Semantics.locals p1 -> MetricLog ->
+             @Semantics.trace p2 -> @Semantics.mem p2 -> @Semantics.locals p2 -> MetricLog ->
+             Prop.
+  Definition ImpSimulation :=
+    forall t1 m1 l1 mc1 t2 m2 l2 mc2 post1,
+      related t1 m1 l1 mc1 t2 m2 l2 mc2 ->
+      exec1 t1 m1 l1 mc1 post1 ->
+      exec2 t2 m2 l2 mc2 (fun t2' m2' l2' mc2' =>
+                            exists t1' m1' l1' mc1',
+                              related t1' m1' l1' mc1' t2' m2' l2' mc2' /\ post1 t1' m1' l1' mc1').
+End TooVerbose.
 
 Section Live.
 
@@ -60,8 +83,11 @@ End Live.
 
 Module map.
   Class ops{K V: Type}(M: map.map K V) := {
-    intersect: M -> M -> M; (* set intersection when interpreting maps as sets of tuples *)
-    default_value: V;
+    (* set intersection when interpreting maps as sets of tuples *)
+    intersect: M -> M -> M;
+    (* for all keys k in (union (dom m1) (dom m2)), applies (f k (get m1 k) (get m2 k))
+       and puts the result in a new map *)
+    combine(m1 m2: M)(f: K -> option V -> option V -> option V): M;
   }.
   Definition putmany_of_pairs{K V: Type}{M: map.map K V}(m: M): list (K * V) -> M :=
     fix rec l :=
@@ -96,7 +122,12 @@ Section RegAlloc.
   Context {srcvar_eq_dec : EqDecider srcvar_eqb}.
   Context {impvar_eq_dec : EqDecider impvar_eqb}.
 
-  Context {src2imp: map.map srcvar impvar}.
+  (* We use the same data structure for mappings from source var to implementation var
+     as well as for deltas of such mappings.
+     If used as mappings, "map.get m x = None" and "map.get m x = Some None" mean the same.
+     If used as deltas, "map.get m x = None" means "no change", and "map.get m x = Some None"
+     means "remove x". *)
+  Context {src2imp: map.map srcvar (option impvar)}.
   Context {src2impOk: map.ok src2imp}.
   Context {src2imp_ops: map.ops src2imp}.
 
@@ -129,29 +160,20 @@ Section RegAlloc.
   Local Notation stmt  := (@FlatImp.stmt srcparams). (* input type *)
   Local Notation stmt' := (@FlatImp.stmt impparams). (* output type *)
 
-  Inductive Update :=
-  | Add(y: impvar)
-  | Remove.
+  (* "Some y" means "put y", "None" means "remove" *)
+  Definition Update := option impvar.
 
-  (* Third case: In "option Update", "None" means unchanged. *)
-
-  Context {Updates: map.map srcvar Update}.
-
-  Definition combine(m1 m2: Updates)(f: srcvar -> option Update -> option Update -> option Update):
-    Updates. Admitted.
-
-  (* should be symmetric *)
   Definition Par1(x: srcvar)(u1: option Update)(u2: option Update): option Update :=
     match u1, u2 with
-    | Some (Add y1), Some (Add y2) => if impvar_eqb y1 y2 then
-                                        Some (Add y1)
+    | Some (Some y1), Some (Some y2) => if impvar_eqb y1 y2 then
+                                        Some (Some y1)
                                       else
-                                        Some Remove
-    | Some (Add y1), Some Remove => Some Remove
-    | Some (Add y1), None => None
-    | Some Remove, _ => Some Remove
-    | None, Some (Add y2) => None
-    | None, Some Remove => Some Remove
+                                        Some None
+    | Some (Some y1), Some None => Some None
+    | Some (Some y1), None => None
+    | Some None, _ => Some None
+    | None, Some (Some y2) => None
+    | None, Some None => Some None
     | None, None => None
     end.
 
@@ -160,53 +182,95 @@ Section RegAlloc.
   Proof.
     intros. destruct u1 as [[? |]|]; destruct u2 as [[? |]|]; try reflexivity.
     simpl.
-    destruct (impvar_eq_dec y y0); destruct (impvar_eq_dec y0 y); congruence.
+    destruct (impvar_eq_dec i i0); destruct (impvar_eq_dec i0 i); congruence.
   Qed.
 
-  Definition Par(us1 us2: Updates): Updates := combine us1 us2 Par1.
-  Definition Seq: Updates -> Updates -> Updates := map.putmany.
+  Lemma Par1_idemp: forall x u,
+      Par1 x u u = u.
+  Proof.
+    intros. unfold Par1. repeat destruct u; simpl; try reflexivity.
+    unfold Update. destruct (impvar_eq_dec i i); try congruence.
+  Qed.
 
-  Definition updates: astmt -> Updates :=
+  Definition Par(us1 us2: src2imp): src2imp := map.combine us1 us2 Par1.
+  Definition Seq: src2imp -> src2imp -> src2imp := map.putmany.
+
+  Axiom combine_idemp: forall f m,
+      (forall k ov, f k ov ov = ov) ->
+      map.combine m m f = m.
+
+  Lemma Par_idemp: forall us,
+      Par us us = us.
+  Proof.
+    intros. unfold Par. apply combine_idemp. intros. apply Par1_idemp.
+  Qed.
+
+  (* loop_inv calculates the mappings which are guaranteed to hold
+     at the beginning of the loop, and
+     loop_updates calculates the delta caused by running the loop from beginning to beginnig
+     any number of times.
+
+     The delta of n loop iterations:
+     0:    map.empty
+     1:    (Seq (updates s1) (updates s2))
+     2:    (Seq (Seq (updates s1) (updates s2)) (Seq (updates s1) (updates s2)))
+           ...
+     i+1:  Seq delta_i (Seq (updates s1) (updates s2))
+
+     Now, since Seq is just `map.putmany`, and `(map.putmany m m) = m`, all delta_i
+     except for i=0 are just `Seq (updates s1) (updates s2)`, and since Par is
+     idempotent and associative, the loop invariant, which should equal
+
+         map.putmany m (infinite_Par delta_0 delta_1 delta_2 ...)
+
+     can instead just be calculated as
+
+         map.putmany m (Par delta_0 delta_1)
+  *)
+  Definition loop_updates(updates: astmt -> src2imp)(s1 s2: astmt): src2imp :=
+    Par map.empty (Seq (updates s1) (updates s2)).
+  Definition loop_inv(updates: astmt -> src2imp)(m: src2imp)(s1 s2: astmt): src2imp :=
+    map.putmany m (loop_updates updates s1 s2).
+
+  Definition updates: astmt -> src2imp :=
     fix rec s :=
       match s with
       | ASLoad _ x x' _ | ASLit x x' _ | ASOp x x' _ _ _ | ASSet x x' _ =>
-           map.put map.empty x (Add x')
+           map.put map.empty x (Some x')
       | ASStore _ _ _ => map.empty
       | ASIf cond s1 s2 => Par (rec s1) (rec s2)
-      | ASLoop s1 cond s2 =>
+      | ASLoop s1 cond s2 => Seq (loop_updates rec s1 s2) (rec s1)
+        (* probably equivalent, but less compatible with checker:
         let r1 := rec s1 in
         let r2 := rec s2 in
         Par r1 (Seq r1 (Seq r2 r1))
+        *)
       | ASSeq s1 s2 => map.putmany (rec s1) (rec s2)
       | ASSkip => map.empty
       | ASInteract binds _ _ | ASCall binds _ _ =>
-           (map.putmany_of_pairs map.empty (List.map (fun '(x, y) => (x, Add y)) binds))
+           (map.putmany_of_pairs map.empty (List.map (fun '(x, y) => (x, Some y)) binds))
       end.
 
-  Definition loop_inv(update: src2imp -> astmt -> src2imp)(m: src2imp)(s1 s2: astmt): src2imp :=
-    map.intersect m (update (update m s1) s2).
+  Definition unwrap_oo{T: Type}(oo: option (option T)): option T :=
+    match oo with
+    | Some o => o
+    | None => None
+    end.
 
-  (* mappings which are guaranteed to hold after executing statement s (under-approximation) *)
-  Definition update: src2imp -> astmt -> src2imp :=
-    fix rec m s :=
-      match s with
-      | ASLoad _ x x' _ | ASLit x x' _ | ASOp x x' _ _ _ | ASSet x x' _ => map.put m x x'
-      | ASStore _ _ _ => m
-      | ASIf cond s1 s2 => map.intersect (rec m s1) (rec m s2)
-      | ASLoop s1 cond s2 => rec (loop_inv rec m s1 s2) s1
-      | ASSeq s1 s2 => rec (rec m s1) s2
-      | ASSkip => m
-      | ASInteract binds _ _ | ASCall binds _ _ => map.putmany_of_pairs m binds
-      end.
+  Definition gett(m: src2imp)(x: srcvar): option impvar := unwrap_oo (map.get m x).
+  Definition putt(m: src2imp)(x: srcvar)(y: impvar): src2imp := map.put m x (Some y).
+
+  Definition gettmany_of_list(m: src2imp)(xs: list srcvar): option (list impvar) :=
+    List.option_all (List.map (gett m) xs).
 
   Definition cond_checker(s2i: src2imp)(cond: @bcond srcparams): option (@bcond impparams) :=
     match cond with
     | CondBinary op x y =>
-        bind_opt x' <- map.get s2i x;
-        bind_opt y' <- map.get s2i y;
+        bind_opt x' <- gett s2i x;
+        bind_opt y' <- gett s2i y;
         Some (CondBinary op x' y')
     | CondNez x =>
-        bind_opt x' <- map.get s2i x;
+        bind_opt x' <- gett s2i x;
         Some (CondNez x')
     end.
 
@@ -214,20 +278,20 @@ Section RegAlloc.
     fix rec m s :=
       match s with
       | ASLoad sz x x' a =>
-          bind_opt a' <- map.get m a;
+          bind_opt a' <- gett m a;
           Some (SLoad sz x' a')
       | ASStore sz a v =>
-          bind_opt a' <- map.get m a;
-          bind_opt v' <- map.get m v;
+          bind_opt a' <- gett m a;
+          bind_opt v' <- gett m v;
           Some (SStore sz a' v')
       | ASLit x x' v =>
           Some (SLit x' v)
       | ASOp x x' op y z =>
-          bind_opt y' <- map.get m y;
-          bind_opt z' <- map.get m z;
+          bind_opt y' <- gett m y;
+          bind_opt z' <- gett m z;
           Some (SOp x' op y' z')
       | ASSet x x' y =>
-          bind_opt y' <- map.get m y;
+          bind_opt y' <- gett m y;
           Some (SSet x' y')
       | ASIf cond s1 s2 =>
           bind_opt cond' <- cond_checker m cond;
@@ -235,22 +299,22 @@ Section RegAlloc.
           bind_opt s2' <- rec m s2;
           Some (SIf cond' s1' s2')
       | ASLoop s1 cond s2 =>
-          let m1 := loop_inv update m s1 s2 in
-          let m2 := update m1 s1 in
-          bind_opt cond' <- cond_checker m2 cond;
+          let m1 := loop_inv updates m s1 s2 in
           bind_opt s1' <- rec m1 s1;
+          let m2 := map.putmany m1 (updates s1) in
+          bind_opt cond' <- cond_checker m2 cond;
           bind_opt s2' <- rec m2 s2;
           Some (SLoop s1' cond' s2')
       | ASSeq s1 s2 =>
           bind_opt s1' <- rec m s1;
-          bind_opt s2' <- rec (update m s1) s2;
+          bind_opt s2' <- rec (map.putmany m (updates s1)) s2;
           Some (SSeq s1' s2')
       | ASSkip => Some SSkip
       | ASCall binds f args =>
-          bind_opt args' <- map.getmany_of_list m args;
+          bind_opt args' <- gettmany_of_list m args;
           Some (SCall (List.map snd binds) f args')
       | ASInteract binds f args =>
-          bind_opt args' <- map.getmany_of_list m args;
+          bind_opt args' <- gettmany_of_list m args;
           Some (SInteract (List.map snd binds) f args')
       end.
 
@@ -293,14 +357,17 @@ Section RegAlloc.
     | _ => ASSkip (* not an assignment *)
     end.
 
+  Variable available_impvars: list impvar.
+  Variable dummy_impvar: impvar.
+
   Definition rename_assignment_lhs(m: src2imp)(x: srcvar)(a: list impvar):
     src2imp * impvar * list impvar :=
-    match map.get m x with
+    match gett m x with
     | Some y => (m, y, a)
     | None   => match a with
-                | y :: rest => (map.put m x y, y, rest)
+                | y :: rest => (putt m x y, y, rest)
                 | nil => (* error: ran out of registers *)
-                  let y := map.default_value in (map.put m x y, y, a)
+                  let y := dummy_impvar in (putt m x y, y, a)
                 end
     end.
 
@@ -312,6 +379,13 @@ Section RegAlloc.
       let '(m, y, a) := rename_assignment_lhs m x a in
       let '(m, res, a) := rename_binds m binds a in
       (m, (x, y) :: res, a)
+    end.
+
+  Definition puttmany_of_pairs(m: src2imp): list (srcvar * impvar) -> src2imp :=
+    fix rec l :=
+    match l with
+    | nil => m
+    | (k, v) :: rest => putt (rec rest) k v
     end.
 
   (* the simplest dumbest possible "register allocator" *)
@@ -339,15 +413,12 @@ Section RegAlloc.
       (m'', ASLoop s1' cond s2', a'')
     | SCall binds f args =>
       let '(m, tuples, a) := rename_binds m binds a in
-      (map.putmany_of_pairs m tuples, ASCall tuples f args, a)
+      (puttmany_of_pairs m tuples, ASCall tuples f args, a)
     | SInteract binds f args =>
       let '(m, tuples, a) := rename_binds m binds a in
-      (map.putmany_of_pairs m tuples, ASInteract tuples f args, a)
+      (puttmany_of_pairs m tuples, ASInteract tuples f args, a)
     | SSkip => (m, ASSkip, a)
     end.
-
-  Variable available_impvars: list impvar.
-  Variable dummy_impvar: impvar.
 
   Fixpoint regalloc
            (m: src2imp)              (* current mapping *)
@@ -357,11 +428,11 @@ Section RegAlloc.
     : astmt :=                       (* annotated statement *)
     match s with
     | SLoad _ x _ | SLit x _ | SOp x _ _ _ | SSet x _ =>
-        match map.get m x with
+        match gett m x with
         | Some y => (* nothing to do because no new interval starts *)
                     annotate_assignment s y
         | None   => (* new interval starts *)
-                    match map.getmany_of_list m usedlater with
+                    match gettmany_of_list m usedlater with
                     | Some used_impvars =>
                       let av := list_diff impvar_eqb available_impvars used_impvars in
                       match av with
@@ -378,7 +449,7 @@ Section RegAlloc.
       ASIf cond s1' s2'
     | SSeq s1 s2 =>
       let s1' := regalloc m s1 (@live srcparams srcvar_eqb s2 usedlater) in
-      let s2' := regalloc (update m s1') s2 usedlater in
+      let s2' := regalloc (map.putmany m (updates s1')) s2 usedlater in
       ASSeq s1' s2'
     | SLoop s1 cond s2 =>
       ASSkip (* TODO *)
@@ -416,7 +487,7 @@ Section RegAlloc.
   Definition register_allocation(s: stmt)(usedlater: list srcvar): option (stmt' * list impvar) :=
     let annotated := regalloc map.empty s usedlater in
     match checker map.empty annotated with
-    | Some res => match map.getmany_of_list (update map.empty annotated) usedlater with
+    | Some res => match gettmany_of_list (updates annotated) usedlater with
                   | Some imp_vars => Some (res, imp_vars)
                   | None => None
                   end
@@ -474,15 +545,53 @@ Section RegAlloc.
       end.
 
   Definition states_compat(st: srcLocals)(m: src2imp)(st': impLocals) :=
-    forall (x: srcvar) (x': impvar),
-      map.get m x = Some x' ->
+    forall (x: srcvar) (y: impvar),
+      gett m x = Some y ->
       forall w,
         map.get st x = Some w ->
-        map.get st' x' = Some w.
+        map.get st' y = Some w.
+
+  Lemma gett_putt_dec: forall r x x' x0,
+      gett (putt r x x') x0 = if srcvar_eqb x x0 then Some x' else gett r x0.
+  Proof.
+    intros. unfold gett, putt, unwrap_oo.
+    rewrite map.get_put_dec.
+    destruct (srcvar_eq_dec x x0); reflexivity.
+  Qed.
+
+  Lemma states_compat_put: forall lH lL v x y r,
+      gett r x = None ->
+      states_compat lH r lL ->
+      states_compat (map.put lH x v) (putt r x y) (map.put lL y v).
+  Proof.
+    unfold states_compat.
+    intros.
+    rewrite (map.get_put_dec (key_eqb := impvar_eqb)).
+    lazymatch goal with
+    | H: map.get (map.put _ _ _) _ = _ |- _ => rewrite map.get_put_dec in H
+    end.
+    lazymatch goal with
+    | H: gett (putt _ _ _) _ = _ |- _ => rewrite gett_putt_dec in H
+    end.
+    destruct_one_match_hyp.
+    - subst x0. replace y0 with y by congruence. replace w with v by congruence.
+      destruct_one_match; congruence.
+    - specialize H0 with (1 := H1) (2 := H2).
+
+      (* problem: two srcvars mapped to the same impvar *)
+  Abort.
+
+  Lemma states_compat_extends: forall st st' r1 r2,
+      map.extends r1 r2 ->
+      states_compat st r1 st' ->
+      states_compat st r2 st'.
+  Proof.
+    unfold states_compat, map.extends.
+  Abort.
 
   Definition precond(m: src2imp)(s: astmt): src2imp :=
     match s with
-    | ASLoop s1 cond s2 => loop_inv update m s1 s2
+    | ASLoop s1 cond s2 => loop_inv updates m s1 s2
     | _ => m
     end.
 
@@ -500,7 +609,7 @@ Section RegAlloc.
 
   Lemma getmany_of_list_states_compat: forall srcnames impnames r lH lL argvals,
       map.getmany_of_list lH srcnames = Some argvals ->
-      map.getmany_of_list r srcnames = Some impnames ->
+      gettmany_of_list r srcnames = Some impnames ->
       states_compat lH r lL ->
       map.getmany_of_list lL impnames = Some argvals.
   Proof.
@@ -509,7 +618,7 @@ Section RegAlloc.
       destruct impnames as [|impname impnames];
       try reflexivity;
       try discriminate;
-      unfold map.getmany_of_list, List.option_all in *; simpl in *;
+      unfold gett, gettmany_of_list, map.getmany_of_list, List.option_all in *; simpl in *;
         repeat (destruct_one_match_hyp; try discriminate).
     simp.
     replace (map.get lL impname) with (Some argval); cycle 1. {
@@ -518,19 +627,18 @@ Section RegAlloc.
     erewrite IHsrcnames; eauto.
   Qed.
 
-  Lemma putmany_of_list_states_compat: forall binds resvals lL lH l' r,
-      map.putmany_of_list (map fst binds) resvals lH = Some l' ->
+  Lemma putmany_of_list_states_compat: forall binds resvals lL lH lH' r,
+      map.putmany_of_list (map fst binds) resvals lH = Some lH' ->
       states_compat lH r lL ->
       exists lL',
         map.putmany_of_list (map snd binds) resvals lL = Some lL' /\
-        states_compat l' (map.putmany_of_pairs r binds) lL'.
+        states_compat lH' (puttmany_of_pairs r binds) lL'.
   Proof.
     induction binds; intros.
     - simpl in H. simp. simpl. eauto.
     - simpl in *. simp.
       specialize IHbinds with (1 := H).
       destruct a as [sv iv].
-      rename l' into lH'.
       apply map.putmany_of_list_sameLength in H.
       rewrite map_length in H. rewrite <- (map_length snd) in H.
       eapply map.sameLength_putmany_of_list in H.
@@ -538,27 +646,46 @@ Section RegAlloc.
       exists lL'. split; [exact H|].
 
   Admitted.
-  (*edestruct IHbinds as (lL' & P & C); cycle 1.
-      + eexists. split; eauto.
-        unfold map.putmany_of_tuples in C.
-*)
 
-  Lemma checker_correct: forall e e' s t m lH mc post,
-      (forall f argnames retnames body,
-          map.get e f = Some (argnames, retnames, body) ->
-          exists args body' annotated binds,
-            map.get e' f = Some (map snd args, map snd binds, body') /\
-            argnames = map fst args /\
-            retnames = map fst binds /\
-            erase annotated = body /\
-            checker (map.putmany_of_pairs map.empty args) annotated = Some body') ->
-      @exec srcSemanticsParams e s t m lH mc post ->
-      forall lL r annotated s',
-      erase annotated = s ->
-      checker r annotated = Some s' ->
+  (* code1  <----erase----  annotated  ----checker---->  code2 *)
+  Definition code_related code1 m code2 := exists annotated,
+      erase annotated = code1 /\ checker m annotated = Some code2.
+
+  Definition envs_related(e1: @env srcSemanticsParams)
+                         (e2: @env impSemanticsParams): Prop :=
+    forall (f: funname) (argnames retnames: list varname) (body1: stmt),
+      map.get e1 f = Some (argnames, retnames, body1) ->
+      exists args body2 binds,
+        map.get e2 f = Some (map snd args, map snd binds, body2) /\
+        argnames = map fst args /\
+        retnames = map fst binds /\
+        code_related body1 (puttmany_of_pairs map.empty args) body2.
+
+  (* requiring states_compat on all mappings which hold might be too strong,
+     we should only require it on all live variables.
+
+     Or use an "unset" command to astmt make sure the current mapping only contains
+     live variables.
+
+     If the checker is correct and succeeds, ...
+
+     What if we have mapping
+     {x1 -> y1}
+     and then update with
+     x7 -> y1
+     --> The "updates" function would have to record "remove by value"!
+ *)
+
+  Lemma checker_correct: forall eH eL,
+      envs_related eH eL ->
+      forall sH t m lH mc post,
+      @exec srcSemanticsParams eH sH t m lH mc post ->
+      forall lL r annotated sL,
+      erase annotated = sH ->
+      checker r annotated = Some sL ->
       states_compat lH (precond r annotated) lL ->
-      @exec impSemanticsParams e' s' t m lL mc (fun t' m' lL' mc' =>
-        exists lH', states_compat lH' (update r annotated) lL' /\
+      @exec impSemanticsParams eL sL t m lL mc (fun t' m' lL' mc' =>
+        exists lH', states_compat lH' (map.putmany r (updates annotated)) lL' /\
                     post t' m' lH' mc').
   Proof.
     induction 2; intros;
@@ -586,6 +713,7 @@ Section RegAlloc.
         simp.
         pose proof putmany_of_list_states_compat as P.
         specialize P with (1 := H3l) (2 := H6). destruct P as (lL' & P & Co). eauto 10.
+(*
 
     - (* SCall *)
       specialize H with (1 := H0). simp.
@@ -594,7 +722,6 @@ Section RegAlloc.
       specialize P with (1 := H2).
       edestruct P as (st0' & Put & Co); cycle 1.
 
-(*
     induction n; intros; [
       match goal with
       | H: eval 0 _ _ _ = Some _ |- _ => solve [inversion H]
@@ -691,21 +818,11 @@ Section RegAlloc.
    *)
   Admitted.
 
-  (* code1  <----erase----  annotated  ----checker---->  code2 *)
-  Definition code_related code1 m code2 := exists annotated,
-      erase annotated = code1 /\ checker m annotated = Some code2.
-
   Definition related: @FlatImp.SimState srcSemanticsParams ->
                       @FlatImp.SimState impSemanticsParams -> Prop :=
     fun '(e1, c1, done1, t1, m1, l1) '(e2, c2, done2, t2, m2, l2) =>
       done1 = done2 /\
-      (forall f argnames retnames body1,
-          map.get e1 f = Some (argnames, retnames, body1) ->
-          exists args body2 binds,
-            map.get e2 f = Some (map snd args, map snd binds, body2) /\
-            argnames = map fst args /\
-            retnames = map fst binds /\
-            code_related body1 (map.putmany_of_pairs map.empty args) body2) /\
+      envs_related e1 e2 /\
       t1 = t2 /\
       m1 = m2 /\
       code_related c1 map.empty c2.
@@ -728,7 +845,7 @@ Section RegAlloc.
       + case TODO_sam.
       + assert (precond map.empty annotated = map.empty) as E by case TODO_sam.
         rewrite E. unfold states_compat. intros.
-        rewrite @map.get_empty in * by typeclasses eauto. discriminate.
+        unfold gett in *. rewrite @map.get_empty in * by typeclasses eauto. discriminate.
     - simpl. intros.
       unfold code_related.
       firstorder idtac.
